Control/Monad/Class/MonadAlt.v
@@ -1,15 +1,17 @@
-Require Import HSLib.Base.
-Require Import Control.Monad.
+Require Export Control.Monad.
 
+(** A monad that models computations which can perform some kind of choice.
+    It may be thought of as nondeterministic choice, which is quite intuitive
+    from the law [bind_choose_l]. *)
 Class MonadAlt (M : Type -> Type) (inst : Monad M) : Type :=
 {
     choose : forall {A : Type}, M A -> M A -> M A;
     choose_assoc :
       forall {X : Type} (a b c : M X),
         choose (choose a b) c = choose a (choose b c);
-    choose_bind_l :
+    bind_choose_l :
       forall (A B : Type) (x y : M A) (f : A -> M B),
         choose x y >>= f = choose (x >>= f) (y >>= f);
 }.
 
-Hint Rewrite @choose_assoc @choose_bind_l : HSLib.
+Hint Rewrite @choose_assoc @bind_choose_l : HSLib.
