Control/Monad/Class/MonadAltR.v
@@ -1,18 +1,17 @@
-Require Import HSLib.Base.
-Require Import Control.Monad.
-Require Import Control.Alternative.
-Require Import Control.Foldable.
+Require Export Control.Monad.
 
+(** Another monad for nondeterministic choice, but it satisfies a different
+    law than [MonadAlt]. *)
 Class MonadAltR (M : Type -> Type) (inst : Monad M) : Type :=
 {
     choose : forall {A : Type}, M A -> M A -> M A;
     choose_assoc :
       forall {X : Type} (a b c : M X),
         choose (choose a b) c = choose a (choose b c);
-    choose_bind_r :
+    bind_choose_r :
       forall (A B : Type) (m : M A) (f g : A -> M B),
-        (m >>= fun x : A => choose (f x) (g x)) =
+        m >>= (fun x : A => choose (f x) (g x)) =
         choose (m >>= f) (m >>= g)
 }.
 
-Hint Rewrite @choose_assoc @choose_bind_r : HSLib.
+Hint Rewrite @choose_assoc @bind_choose_r : HSLib.
