Control/Monad/Class/MonadAltSet.v
@@ -1,8 +1,7 @@
-Require Import HSLib.Base.
-Require Import Control.Monad.
+Require Export Control.Monad.
 
-(** The initial model are finite bags
-    (which probably means finite multisets). *)
+(** A nondeterministic choice monad whose initial model are finite sets.
+    This is guaranteed by the laws [choose_comm] and [choose_idempotent]. *)
 Class MonadAltSet (M : Type -> Type) (inst : Monad M) : Type :=
 {
     choose : forall {A : Type}, M A -> M A -> M A;
