Control/Monad/Class/MonadFree.v
@@ -1,6 +1,6 @@
-Require Import HSLib.Base.
-Require Import Control.Monad.
+Require Export Control.Monad.
 
+(** A class that represents a free monad of a functor [F]. *)
 Class MonadFree
   (F M : Type -> Type) (instF : Functor F) (instM : Monad M) : Type :=
 {
@@ -10,6 +10,5 @@ Class MonadFree
         wrap (fmap f x) = wrap (@fmap F instF _ _ pure x) >>= f
 }.
 
-(*
-Hint Rewrite @wrap_law : HSLib.
-*)
+(** There's no rewrite hint for [wrap_law], because it can be rewritten
+    ad infinitum, so [autorewrite] would loop. *)
