Control/Monad/Class/MonadStateNondet.v
@@ -1,9 +1,9 @@
-Require Import HSLib.Base.
-Require Import Control.Monad.
+Require Export Control.Monad.Class.MonadNondet.
+Require Export Control.Monad.Class.MonadState.
 
-Require Import Control.Monad.Class.MonadNondet.
-Require Import Control.Monad.Class.MonadState.
-
+(** A monad that models both nondeterministic and stateful computations.
+    
+*)
 Class MonadStateNondet
   (S : Type) (M : Type -> Type) (inst : Monad M) : Type :=
 {
@@ -12,7 +12,7 @@ Class MonadStateNondet
     seq_fail_r :
       forall (A B : Type) (x : M A),
         x >> fail = @fail M inst instN B;
-    bind_choose_distr :
+    bind_choose_r :
       forall (A B : Type) (f g : A -> M B) (ma : M A),
         ma >>= (fun x : A => choose (f x) (g x)) =
         choose (ma >>= f) (ma >>= g)
@@ -21,4 +21,4 @@ Class MonadStateNondet
 Coercion instS : MonadStateNondet >-> MonadState.
 Coercion instN : MonadStateNondet >-> MonadNondet.
 
-Hint Rewrite @seq_fail_r @bind_choose_distr : HSLib.
+Hint Rewrite @seq_fail_r @bind_choose_r : HSLib.
